feat: mem_ext

Arithmetization/Bit.lean
@@ -1,4 +1,5 @@
 import Arithmetization.Exponential.Exp
+import Arithmetization.Exponential.Log
 
 namespace LO.FirstOrder
 
@@ -6,14 +7,11 @@ namespace Arith
 
 noncomputable section
 
-variable {M : Type} [Inhabited M] [DecidableEq M] [ORingSymbol M]
-  [Structure ℒₒᵣ M] [Structure.ORing ℒₒᵣ M]
-  [𝐏𝐀⁻.Mod M]
+variable {M : Type} [Zero M] [One M] [Add M] [Mul M] [LT M] [𝐏𝐀⁻.Mod M]
 
 namespace Model
 
 variable [𝐈𝚺₁.Mod M]
-
 
 def Bit (i a : M) : Prop := LenBit (exp i) a
 
@@ -83,16 +81,30 @@ lemma not_mem_iff_mul_exp_add {i a : M} : i ∉ a ↔ ∃ k, ∃ r < exp i, a = 
   · simpa [exponential_inj.eq_iff] using
       lenbit_add_pow2_iff_of_not_lenbit (exp_pow2 i) (exp_pow2 j) h
 
+lemma pos_of_nonempty {i a : M} (h : i ∈ a) : 0 < a := by
+  by_contra A; simp at A; rcases A; simp_all
+
+lemma log_mem_of_pos {a : M} (h : 0 < a) : log a ∈ a :=
+  mem_iff_mul_exp_add_exp_add.mpr
+    ⟨0, a - exp log a,
+      (tsub_lt_iff_left (exponential_log_le_self h)).mpr (by rw [←two_mul]; exact lt_two_mul_exponential_log h),
+      by simp; exact Eq.symm <| add_tsub_self_of_le (exponential_log_le_self h)⟩
+
+lemma le_log_of_mem {i a : M} (h : i ∈ a) : i ≤ log a := (exp_le_iff_le_log (pos_of_nonempty h)).mp (exp_le_of_mem h)
+
+lemma succ_mem_iff_mem_div_two {i a : M} : i + 1 ∈ a ↔ i ∈ a / 2 := by simp [mem_iff_bit, Bit, LenBit.iff_rem, exp_succ, div_mul]
+
+lemma lt_binary_length_of_mem {i a : M} (h : i ∈ a) : i < ‖a‖ := by
+  simpa [binary_length_of_pos (pos_of_nonempty h), ←le_iff_lt_succ] using le_log_of_mem h
+
 lemma lt_exp_iff {a i : M} : a < exp i ↔ ∀ j ∈ a, j < i :=
   ⟨fun h j hj ↦ exponential_monotone.mp <| lt_of_le_of_lt (exp_le_of_mem hj) h,
-  by {
-    contrapose; simp
-    intro (h : exp i ≤ a)
+   by contrapose; simp
+      intro (h : exp i ≤ a)
+      have pos : 0 < a := lt_of_lt_of_le (by simp) h
+      exact ⟨log a, log_mem_of_pos pos, (exp_le_iff_le_log pos).mp h⟩⟩
 
-
-   }⟩
-
-instance : HasSubset M := ⟨fun a b ↦ ∀ {i}, i ∈ a → i ∈ b⟩
+instance : HasSubset M := ⟨fun a b ↦ ∀ ⦃i⦄, i ∈ a → i ∈ b⟩
 
 def bitSubsetdef : Σᴬ[0] 2 := ⟨“∀[#0 < #1] (!bitdef [#0, #1] → !bitdef [#0, #2])”, by simp⟩
 
@@ -102,13 +114,69 @@ lemma bitSubset_defined : Σᴬ[0]-Relation ((· ⊆ ·) : M → M → Prop) bit
 
 instance {b s} : DefinableRel b s ((· ⊆ ·) : M → M → Prop) := defined_to_with_param₀ _ bitSubset_defined
 
+lemma mem_exp_add_succ_sub_one (i j : M) : i ∈ exp (i + j + 1) - 1 := by
+  have : exp (i + j + 1) - 1 = (exp j - 1) * exp (i + 1) + exp i + (exp i - 1) := calc
+    exp (i + j + 1) - 1 = exp j * exp (i + 1) - 1                             := by simp [exp_add, ←mul_assoc, mul_comm]
+    _                   = exp j * exp (i + 1) - exp (i + 1) + exp (i + 1) - 1 := by rw [sub_add_self_of_le]; exact le_mul_of_pos_left (exp_pos j)
+    _                   = (exp j - 1) * exp (i + 1) + exp (i + 1) - 1         := by simp [sub_mul]
+    _                   = (exp j - 1) * exp (i + 1) + (exp i + exp i) - 1     := by simp [←two_mul, ←exp_succ i]
+    _                   = (exp j - 1) * exp (i + 1) + (exp i + exp i - 1)     := by rw [add_tsub_assoc_of_le]; simp [←two_mul, ←pos_iff_one_le]
+    _                   = (exp j - 1) * exp (i + 1) + exp i + (exp i - 1)     := by simp [add_assoc, add_tsub_assoc_of_le]
+  exact mem_iff_mul_exp_add_exp_add.mpr ⟨exp j - 1, exp i - 1, (tsub_lt_iff_left (by simp)).mpr $ by simp, this⟩
+
+/-- under a = {0, 1, 2, ..., a - 1} -/
+def under (a : M) : M := exp a - 1
+
+lemma mem_under_iff {i j : M} : i ∈ under j ↔ i < j := by
+  constructor
+  · intro h
+    have : exp i < exp j := calc
+      exp i ≤ exp j - 1 := exp_le_of_mem h
+      _     < exp j     := pred_lt_self_of_pos (exp_pos j)
+    exact exponential_monotone.mp this
+  · intro lt
+    have := lt_iff_succ_le.mp lt
+    let k := j - (i + 1)
+    have : j = i + k + 1 := by
+      simp [add_assoc, ←sub_sub]; rw [sub_add_self_of_le, add_tsub_self_of_le]
+      · exact le_of_lt lt
+      · exact le_tsub_of_add_le_left this
+    rw [this]; exact mem_exp_add_succ_sub_one i k
+
+lemma eq_zero_of_subset_zero {a : M} : a ⊆ 0 → a = 0 := by
+  intro h; by_contra A
+  have : log a ∈ 0 := h (log_mem_of_pos (pos_iff_ne_zero.mpr A))
+  simp_all
+
+lemma subset_div_two {a b : M} : a ⊆ b → a / 2 ⊆ b / 2 := by
+  intro ss i hi
+  have : i + 1 ∈ a := succ_mem_iff_mem_div_two.mpr hi
+  exact succ_mem_iff_mem_div_two.mp <| ss this
+
+lemma zero_mem_iff {a : M} : 0 ∉ a ↔ 2 ∣ a := by simp [mem_iff_bit, Bit, LenBit]
+
+@[simp] lemma zero_not_mem (a : M) : 0 ∉ 2 * a := by simp [mem_iff_bit, Bit, LenBit]
+
 lemma le_of_subset {a b : M} (h : a ⊆ b) : a ≤ b := by
-  by_contra A
+  revert a
+  induction b using hierarchy_polynomial_induction_pi₁
+  · definability
+  case zero =>
+    intro a h
+    simp [eq_zero_of_subset_zero h]
+  case even b IH =>
+    intro a ha
+    have IH : a / 2 ≤ b := IH (by simpa using subset_div_two ha)
+    have : 2 * (a / 2) = a :=
+      mul_div_self_of_dvd.mpr (zero_mem_iff.mp $ by intro h; have : 0 ∈ 2 * b := ha h; simp_all)
+    simpa [this] using mul_le_mul_left (a := 2) IH
+  case odd b IH =>
+    intro a ha
+    have IH : a / 2 ≤ b := IH (by simpa [div_mul_add' b 2 one_lt_two] using subset_div_two ha)
+    exact le_trans (le_two_mul_div_two_add_one a) (by simpa using IH)
 
-
-lemma mem_ext {a b : M} (h : ∀ i, i ∈ a ↔ i ∈ b) : a = b := by sorry
-
-
+lemma mem_ext {a b : M} (h : ∀ i, i ∈ a ↔ i ∈ b) : a = b :=
+  le_antisymm (le_of_subset $ fun i hi ↦ (h i).mp hi) (le_of_subset $ fun i hi ↦ (h i).mpr hi)
 
 end Model
 
